StructuredEncryption/test/Paths.dfy
@@ -1,0 +1,134 @@
+// Copyright Amazon.com Inc. or its affiliates. All Rights Reserved.
+// SPDX-License-Identifier: Apache-2.0
+include "../src/Paths.dfy"
+
+module PathsTests {
+  import opened Wrappers
+  import opened StandardLibrary
+  import opened StandardLibrary.UInt
+  import opened Paths
+
+  // This first part converts strings to TerminalLocations
+  // It will be moved to src/Paths when we do Beacons 
+
+  // return the number of characters until the next part begins
+  // that is, '[' or '.'
+  function method  {:opaque} FindStartOfNext(s : string)
+    : (index : Option<nat>)
+    ensures index.Some? ==> 
+      && index.value < |s|
+      && (s[index.value] == '.' || s[index.value] == '[')
+      && '.' !in s[..index.value]
+      && '[' !in s[..index.value]
+    ensures index.None? ==> '.' !in s && '[' !in s
+  {
+    var dot := FindIndexMatching(s, '.', 0);
+    var bracket := FindIndexMatching(s, '[', 0);
+    if dot.None? && bracket.None? then
+      None
+    else if dot.Some? && bracket.Some? then
+      if dot.value < bracket.value then
+        dot
+      else
+        bracket
+    else if dot.Some? then
+      dot
+    else
+      bracket
+  }
+
+  // read an unsigned decomal number, return value and length
+  function method {:tailrecursion} {:opaque} GetNumber(s : string, acc : nat := 0)
+    : Result<nat, string>
+  {
+    if |s| == 0 then
+      Success(acc)
+    else if '0' <= s[0] <= '9' then
+      GetNumber(s[1..], acc * 10 + s[0] as nat - '0' as nat)
+    else
+      Failure("Unexpected character in number : " + [s[0]])
+  }
+
+  // make Map from string
+  function method  {:opaque} MakeMap(s : string) : (ret : Result<Selector, string>)
+    ensures ret.Success? ==> ret.value.Map?
+  {
+    :- Need(ValidString(s), "Key string invalid.");
+    Success(Map(s))
+  }
+
+  // convert string to Selector
+  function method {:opaque} GetSelector(s : string)
+    : Result<Selector, string>
+    requires |s| > 0 && (s[0] == '.' || s[0] == '[')
+  {
+    if s[0] == '.' then
+      var m :- MakeMap(s[1..]);
+      Success(m)
+    else
+      if s[|s|-1] != ']' then
+        Failure("List index must end with ]")
+      else
+        var num :- GetNumber(s[1..|s|-1]);
+        :- Need(num < UINT64_LIMIT, "Array selector exceeds maximum.");
+        Success(List(num as uint64))
+  }
+
+  // convert string to SelectorList
+  function method {:tailrecusrion} {:opaque} GetSelectors(s : string, acc : SelectorList := [])
+    : Result<SelectorList, string>
+    requires |s| > 0 && (s[0] == '.' || s[0] == '[')
+  {
+    var pos := FindStartOfNext(s[1..]);
+    var end := if pos.None? then |s| else pos.value + 1;
+    var sel : Selector :- GetSelector(s[..end]);
+    :- Need(|acc|+1 < UINT64_LIMIT, "Selector Overflow");
+    if pos.None? then
+      Success(acc + [sel])
+    else
+      GetSelectors(s[end..], acc + [sel])
+  }
+
+  // convert string to TerminalLocation
+  function method {:opaque} MakeTerminalLocation(s : string)
+    : (ret : Result<TerminalLocation, string>)
+    ensures ret.Success? ==> 0 < |ret.value.parts|
+  {
+    :- Need(0 < |s|, "Path specification must not be empty.");
+    var pos := FindStartOfNext(s);
+    if pos.None? then
+      var m :- MakeMap(s);
+      Success(TerminalLocation([m]))
+    else
+      var name := s[..pos.value];
+      var selectors :- GetSelectors(s[pos.value..]);
+      var m :- MakeMap(name);
+      :- Need(|selectors|+1 < UINT64_LIMIT, "Selector Overflow");
+      Success(TerminalLocation([m] + selectors))
+  }
+
+  method {:test} TestSpecExamples() {
+    var tableName : GoodString := "example_table";
+    assert(ValidString("example_table"));
+    var nameSrc :- expect MakeTerminalLocation("name");
+    expect nameSrc.canonicalPath(tableName) == 
+         UTF8.EncodeAscii("example_table")
+      + [0,0,0,0,0,0,0,1] // depth
+      + ['$' as uint8] // map
+      + [0,0,0,0,0,0,0,4] // length
+      + UTF8.EncodeAscii("name");
+
+    var stampSrc :- expect MakeTerminalLocation("status-history[0].timestamp");
+    expect stampSrc.canonicalPath(tableName) == 
+        UTF8.EncodeAscii("example_table")
+      + [0,0,0,0,0,0,0,3] // depth
+      + ['$' as uint8] // map
+      + [0,0,0,0,0,0,0,14] // length of "status-history"
+      + UTF8.EncodeAscii("status-history")
+      + ['#' as uint8] // array
+      + [0,0,0,0,0,0,0,0] // index
+      + ['$' as uint8] // map
+      + [0,0,0,0,0,0,0,9] // length of "timestamp"
+      + UTF8.EncodeAscii("timestamp");
+  }
+}
